type/step.v
@@ -420,6 +420,227 @@ Proof.
 Qed.
 
 
+Lemma wfgC_after_step_helper : forall n0 s G' lsg lis1, 
+      Some (s, G') = onth n0 lsg -> 
+      Forall2
+       (fun (u : option (sort * global)) (v : option (sort * gtt)) =>
+        u = None /\ v = None \/
+        (exists (s : sort) (g : global) (g' : gtt),
+           u = Some (s, g) /\ v = Some (s, g') /\ upaco2 gttT bot2 g g')) lis1 lsg -> 
+      Forall
+       (fun u : option (sort * global) =>
+        u = None \/ (exists (s : sort) (g : global), u = Some (s, g) /\ wfG g)) lis1 -> 
+      Forall
+      (fun u : option (sort * gtt) =>
+       u = None \/ (exists (s : sort) (g : gtt), u = Some (s, g) /\ balancedG g)) lsg -> 
+      Forall
+       (fun u : option (sort * global) =>
+        u = None \/
+        (exists (s : sort) (g : global),
+           u = Some (s, g) /\ (forall n : fin, exists m : fin, guardG n m g))) lis1 -> 
+      exists G1, onth n0 lis1 = Some(s, G1) /\ gttTC G1 G' /\ wfG G1 /\ balancedG G' /\ (forall n, exists m, guardG n m G1).
+Proof.
+  induction n0; intros.
+  - destruct lsg; try easy. destruct lis1; try easy.
+    inversion H0. subst. clear H0. inversion H1. subst. clear H1. inversion H2. subst. clear H2.
+    inversion H3. subst. clear H3. 
+    simpl in H. subst.
+    destruct H7; try easy. destruct H as (s0,(g1,(g2,(Ha,(Hb,Hc))))). inversion Hb. subst.
+    destruct H5; try easy. destruct H as (s1,(g3,(Hd,He))). inversion Hd. subst.
+    destruct H4; try easy. destruct H as (s2,(g4,(Hf,Hg))). inversion Hf. subst.
+    destruct H2; try easy. destruct H as (s3,(g5,(Hh,Hi))). inversion Hh. subst.
+    simpl. exists g5. pclearbot. easy.
+  - destruct lsg; try easy. destruct lis1; try easy.
+    inversion H0. subst. clear H0. inversion H1. subst. clear H1. inversion H2. subst. clear H2.
+    inversion H3. subst. clear H3. 
+    specialize(IHn0 s G' lsg lis1). apply IHn0; try easy.
+Qed.
+
+Lemma wfgC_after_step_helper2 : forall lis ys ys0 n p q,
+    SList lis -> 
+    Forall2
+       (fun (u : option (sort * global)) (v : option (sort * gtt)) =>
+        u = None /\ v = None \/
+        (exists (s : sort) (g : global) (g' : gtt),
+           u = Some (s, g) /\ v = Some (s, g') /\ upaco2 gttT bot2 g g')) lis ys -> 
+    Forall2
+        (fun u v : option (sort * gtt) =>
+         u = None /\ v = None \/
+         (exists (s : sort) (g g' : gtt),
+            u = Some (s, g) /\ v = Some (s, g') /\ upaco5 gttstep bot5 g g' p q n))
+        ys ys0 ->
+    SList ys0.
+Proof.
+  induction lis; intros; try easy.
+  specialize(SList_f a lis H); intros. destruct ys; try easy. destruct ys0; try easy.
+  specialize(IHlis ys ys0 n p q). inversion H0. subst. clear H0. inversion H1. subst. clear H1.
+  destruct H2. apply SList_b. apply IHlis; try easy.
+  destruct H0. destruct H1. subst. destruct H6; try easy.
+  destruct H0 as (s0,(g0,(g1,(Ha,(Hb,Hc))))). subst. destruct ys; try easy.
+  destruct H5; try easy. destruct H0 as (s2,(g2,(g3,(Hta,(Htb,Htc))))). inversion Hta. subst.
+  destruct ys0; try easy.
+Qed.
+
+Lemma wfgC_after_step_helper3 : forall ys0 xs,
+      SList ys0 -> 
+      Forall2
+       (fun (u : option (sort * global)) (v : option (sort * gtt)) =>
+        u = None /\ v = None \/
+        (exists (s : sort) (g : global) (g' : gtt),
+           u = Some (s, g) /\ v = Some (s, g') /\ gttTC g g')) xs ys0 -> 
+      SList xs.
+Proof.
+  induction ys0; intros; try easy.
+  specialize(SList_f a ys0 H); intros. 
+  destruct xs; try easy.
+  specialize(IHys0 xs). inversion H0. subst. clear H0.
+  destruct H1. apply SList_b. apply IHys0; try easy.
+  destruct H0. destruct H1. subst.
+  destruct H5; try easy. destruct H0 as (s,(g,(g',(Ha,(Hb,Hc))))). inversion Hb. subst.
+  destruct xs; try easy.
+Qed.
+
+
+Theorem wfgCw_after_step : forall G G' p q n, wfgC G -> gttstepC G G' p q n -> wfgCw G'. 
+Proof.
+  intros. 
+  pose proof H as Ht. unfold wfgC in H.
+  destruct H as (Gl,(Ha,(Hb,(Hc,Hd)))).
+  specialize(wfgC_step_part G G' p q n Ht H0); intros.
+  specialize(balanced_to_tree G p Ht H); intros. clear Ht H.
+  destruct H1 as (Gt,(ctxG,(Hta,(Htb,(Htc,Htd))))).
+  clear Htd.
+  revert Htc Htb Hta H0 Hd Hc Hb Ha.
+  revert G G' p q n Gl ctxG.
+  induction Gt using gtth_ind_ref; intros; try easy.
+  - inversion Hta. subst.
+    specialize(Forall_forall (fun u : option gtt =>
+         u = None \/
+         (exists (q : string) (lsg : seq.seq (option (sort * gtt))),
+            u = Some (gtt_send p q lsg) \/
+            u = Some (gtt_send q p lsg) \/ u = Some gtt_end)) ctxG); intros.
+    destruct H. specialize(H Htc). clear H1 Htc.
+    specialize(some_onth_implies_In n ctxG G H2); intros.
+    specialize(H (Some G) H1). destruct H; try easy. destruct H as (r,(lsg,Hsa)). clear H1.
+    - destruct Hsa. inversion H. subst. 
+      pinversion H0; try easy. subst. clear H6 H.
+      specialize(guard_breakG_s2 (gtt_send p q lsg) Gl Hc Hb Ha); intros.
+      clear Ha Hb Hc. clear Gl. destruct H as (Gl,(Ha,(Hb,(Hc,He)))).
+      destruct Ha. subst. pinversion He. apply gttT_mon.
+      destruct H as (p1,(q1,(lis1,H))). subst. pinversion He; try easy. subst.
+      inversion Hc. subst.
+      specialize(balanced_cont Hd); intros.
+      specialize(guard_cont Hb); intros.
+      specialize(wfgC_after_step_helper n0 s G' lsg lis1); intros.
+      assert(exists G1 : global,
+       onth n0 lis1 = Some (s, G1) /\
+       gttTC G1 G' /\
+       wfG G1 /\ balancedG G' /\ (forall n : fin, exists m : fin, guardG n m G1)).
+      apply H4; try easy. clear H4. clear H3 H H7 H1.
+      destruct H8 as (G1,(Hsa,(Hsb,(Htc,(Htd,Hte))))). exists G1. easy.
+      apply gttT_mon.
+      apply step_mon.
+    - destruct H. inversion H. subst. pinversion H0; try easy. apply step_mon.
+    - inversion H. subst. pinversion H0; try easy. apply step_mon.
+  - inversion Hta. subst.
+    assert(wfgC (gtt_send p q ys)).
+    {
+      unfold wfgC. exists Gl. easy.
+    }
+    rename H1 into Ht.
+    pinversion H0; try easy.
+    - subst. assert False. apply Htb. constructor. easy.
+    subst. rename p into s. rename q into s'. rename p0 into p. rename q0 into q.
+    specialize(guard_breakG_s2 (gtt_send s s' ys) Gl Hc Hb Ha); intros. clear Ha Hb Hc. clear Gl.
+    destruct H1 as (Gl,(Ha,(Hb,(Hc,He)))). destruct Ha. subst. pinversion He; try easy. apply gttT_mon.
+    destruct H1 as (p1,(q1,(lis,H1))). subst. pinversion He; try easy. subst. inversion Hc. subst.
+    specialize(balanced_cont Hd); intros.
+    specialize(guard_cont Hb); intros.
+    assert(List.Forall (fun u => u = None \/ (exists s g, u = Some (s, g) /\ wfgCw g)) ys0).
+    {
+      clear H14 H13 Hb Hc He H16 H11 H10 H9 H8 H5 H4 H6 Hta H0 Hd.
+      apply Forall_forall; intros. 
+      destruct x.
+      - specialize(in_some_implies_onth p0 ys0 H0); intros. destruct H4 as (n0 ,H4). clear H0.
+        right. destruct p0. exists s0. exists g. split. easy.
+        clear Ht.
+        revert H4 H3 H1 H15 H2 H17 H7 Htc H Htb.
+        revert g s0 lis ys ys0 ctxG n p q xs s s'.
+        induction n0; intros.
+        - destruct ys0; try easy. destruct ys; try easy. destruct lis; try easy.
+          destruct xs; try easy.
+          inversion H3. subst. clear H3. inversion H1. subst. clear H1. inversion H15. subst. clear H15.
+          inversion H2. subst. clear H2. inversion H17. subst. clear H17. inversion H7. subst. clear H7.
+          inversion H. subst. clear H.
+          clear H8 H9 H10 H14 H15 H17 H7.
+          simpl in H4. subst.
+          destruct H11; try easy. destruct H as (s1,(g1,(g2,(Ha,(Hb,Hc))))). inversion Hb. subst.
+          destruct H13; try easy. destruct H as (s2,(g3,(g4,(Hd,(He,Hf))))). inversion He. subst.
+          destruct H12; try easy. destruct H as (s3,(g5,(g6,(Hg,(Hh,Hi))))). inversion Hh. subst.
+          destruct H3; try easy. destruct H as (s4,(g7,(Hj,Hk))). inversion Hj. subst.
+          destruct H6; try easy. destruct H as (s5,(g8,(Hl,Hm))). inversion Hl. subst.
+          destruct H5; try easy. destruct H as (s6,(g9,(Hn,Ho))). inversion Hn. subst.
+          destruct H2; try easy. clear Hn Hh He Hj Hl Hb.
+          destruct H as (s7,(g10,(Hp,Hq))). inversion Hp. subst.
+          specialize(Hq g9 g2 p q n g8 ctxG).
+          apply Hq; try easy. 
+          specialize(ishParts_x Htb); try easy.
+          destruct Hc; try easy.
+          destruct Hi; try easy. 
+        - destruct ys0; try easy. destruct ys; try easy. destruct lis; try easy.
+          destruct xs; try easy.
+          inversion H3. subst. clear H3. inversion H1. subst. clear H1. inversion H15. subst. clear H15.
+          inversion H2. subst. clear H2. inversion H17. subst. clear H17. inversion H7. subst. clear H7.
+          inversion H. subst. clear H. 
+          specialize(IHn0 g s0 lis ys ys0 ctxG n p q xs s s').
+          apply IHn0; try easy.
+          specialize(ishParts_hxs Htb); try easy.
+        left. easy.
+    }
+    specialize(wfgC_after_step_helper2 lis ys ys0 n p q H13 H2 H17); intros.
+    assert(wfgC (gtt_send s s' ys) /\ gttstepC (gtt_send s s' ys) (gtt_send s s' ys0) p q n). 
+    {
+      unfold wfgC. split. exists (g_send s s' lis). split. pfold. easy. easy.
+      pfold. easy.
+    }
+    destruct H19.
+    clear H3 H1 H15 H2 Hb Hc He H17 H16 H11 H10 H9 H8 H5 H4 H7 Hta H0 Hd Htb Htc H H6 H13. clear Ht H19 H20.
+    clear p q xs n ctxG ys lis. rename H14 into H. rename H12 into H1.
+    assert(exists xs, List.Forall2 (fun u v => (u = None /\ v = None) \/ (exists s g g', u = Some(s, g) /\ v = Some(s, g') /\ gttTC g g')) xs ys0 /\ 
+    List.Forall (fun u => u = None \/ (exists s g, u = Some(s, g) /\ wfG g)) xs /\
+    List.Forall (fun u => u = None \/ (exists s g, u = Some(s, g) /\ (forall n, exists m, guardG n m g))) xs).
+    {
+      clear H. revert H1. clear H18. revert ys0. clear s s'.
+      induction ys0; intros; try easy.
+      - exists nil. easy.
+      - inversion H1. subst. clear H1.
+        specialize(IHys0 H3). destruct IHys0 as (xs,H).
+        destruct H2. 
+        - subst. exists (None :: xs).
+          split. constructor; try easy. left. easy.
+          split. constructor; try easy. left. easy.
+          constructor; try easy. left. easy.
+        - destruct H0 as (s,(g,(Ha,Hb))). subst.
+          unfold wfgC in Hb. destruct Hb.
+          exists (Some(s, x) :: xs).
+          split. constructor; try easy. right. exists s. exists x. exists g. easy.
+          split. constructor; try easy. right. exists s. exists x. easy.
+          constructor; try easy. right. exists s. exists x. easy.
+    }
+    destruct H0 as (xs,(Ha,(Hb,Hc))).
+    exists (g_send s s' xs).
+    - split. pfold. constructor; try easy.
+      revert Ha. apply Forall2_mono; intros; try easy. destruct H0. left. easy.
+      destruct H0 as (s0,(g0,(g1,(Hta,(Htb,Htc))))). subst. right. exists s0. exists g0. exists g1. 
+      split. easy. split. easy. left. easy.
+    - split. constructor; try easy.
+      specialize(wfgC_after_step_helper3 ys0 xs H18 Ha); try easy.
+    - apply guard_cont_b; try easy.
+    apply gttT_mon.
+    apply step_mon.
+Qed.
+
+
 
 
 
