type/wfgC_after_step.v
@@ -5,100 +5,455 @@ From Paco Require Import paco pacotac.
 Require Import Setoid Morphisms Coq.Program.Basics.
 Require Import Coq.Init.Datatypes.
 
-Lemma wfgC_after_step_helper : forall n0 s G' lsg lis1, 
-      Some (s, G') = onth n0 lsg -> 
-      Forall2
-       (fun (u : option (sort * global)) (v : option (sort * gtt)) =>
-        u = None /\ v = None \/
-        (exists (s : sort) (g : global) (g' : gtt),
-           u = Some (s, g) /\ v = Some (s, g') /\ upaco2 gttT bot2 g g')) lis1 lsg -> 
-      Forall
-       (fun u : option (sort * global) =>
-        u = None \/ (exists (s : sort) (g : global), u = Some (s, g) /\ wfG g)) lis1 -> 
-      Forall
-      (fun u : option (sort * gtt) =>
-       u = None \/ (exists (s : sort) (g : gtt), u = Some (s, g) /\ balancedG g)) lsg -> 
-      Forall
-       (fun u : option (sort * global) =>
-        u = None \/
-        (exists (s : sort) (g : global),
-           u = Some (s, g) /\ (forall n : fin, exists m : fin, guardG n m g))) lis1 -> 
-      exists G1, onth n0 lis1 = Some(s, G1) /\ gttTC G1 G' /\ wfG G1 /\ balancedG G' /\ (forall n, exists m, guardG n m G1).
-Proof.
-  induction n0; intros.
-  - destruct lsg; try easy. destruct lis1; try easy.
-    inversion H0. subst. clear H0. inversion H1. subst. clear H1. inversion H2. subst. clear H2.
-    inversion H3. subst. clear H3. 
-    simpl in H. subst.
-    destruct H7; try easy. destruct H as (s0,(g1,(g2,(Ha,(Hb,Hc))))). inversion Hb. subst.
-    destruct H5; try easy. destruct H as (s1,(g3,(Hd,He))). inversion Hd. subst.
-    destruct H4; try easy. destruct H as (s2,(g4,(Hf,Hg))). inversion Hf. subst.
-    destruct H2; try easy. destruct H as (s3,(g5,(Hh,Hi))). inversion Hh. subst.
-    simpl. exists g5. pclearbot. easy.
-  - destruct lsg; try easy. destruct lis1; try easy.
-    inversion H0. subst. clear H0. inversion H1. subst. clear H1. inversion H2. subst. clear H2.
-    inversion H3. subst. clear H3. 
-    specialize(IHn0 s G' lsg lis1). apply IHn0; try easy.
-Qed.
 
-Lemma wfgC_after_step_helper2 : forall lis ys ys0 n p q,
-    SList lis -> 
-    Forall2
-       (fun (u : option (sort * global)) (v : option (sort * gtt)) =>
-        u = None /\ v = None \/
-        (exists (s : sort) (g : global) (g' : gtt),
-           u = Some (s, g) /\ v = Some (s, g') /\ upaco2 gttT bot2 g g')) lis ys -> 
-    Forall2
-        (fun u v : option (sort * gtt) =>
-         u = None /\ v = None \/
-         (exists (s : sort) (g g' : gtt),
-            u = Some (s, g) /\ v = Some (s, g') /\ upaco5 gttstep bot5 g g' p q n))
-        ys ys0 ->
-    SList ys0.
-Proof.
-  induction lis; intros; try easy.
-  specialize(SList_f a lis H); intros. destruct ys; try easy. destruct ys0; try easy.
-  specialize(IHlis ys ys0 n p q). inversion H0. subst. clear H0. inversion H1. subst. clear H1.
-  destruct H2. apply SList_b. apply IHlis; try easy.
-  destruct H0. destruct H1. subst. destruct H6; try easy.
-  destruct H0 as (s0,(g0,(g1,(Ha,(Hb,Hc))))). subst. destruct ys; try easy.
-  destruct H5; try easy. destruct H0 as (s2,(g2,(g3,(Hta,(Htb,Htc))))). inversion Hta. subst.
-  destruct ys0; try easy.
-Qed.
-
-Lemma wfgC_after_step_helper3 : forall ys0 xs,
-      SList ys0 -> 
-      Forall2
-       (fun (u : option (sort * global)) (v : option (sort * gtt)) =>
-        u = None /\ v = None \/
-        (exists (s : sort) (g : global) (g' : gtt),
-           u = Some (s, g) /\ v = Some (s, g') /\ gttTC g g')) xs ys0 -> 
-      SList xs.
-Proof.
-  induction ys0; intros; try easy.
-  specialize(SList_f a ys0 H); intros. 
-  destruct xs; try easy.
-  specialize(IHys0 xs). inversion H0. subst. clear H0.
-  destruct H1. apply SList_b. apply IHys0; try easy.
-  destruct H0. destruct H1. subst.
-  destruct H5; try easy. destruct H0 as (s,(g,(g',(Ha,(Hb,Hc))))). inversion Hb. subst.
-  destruct xs; try easy.
-Qed.
-
-
-(* hint : induction on balanced_to_tree *)
-Lemma step_gtth : forall G G' p q l,
+Lemma proj_cont_pq_step : forall G G' p q l,
     wfgC G -> 
     gttstepC G G' p q l -> 
-    exists ctxG ctxG2 Gl, typ_gtth ctxG Gl G /\ typ_gtth ctxG2 Gl G' /\
-    (ishParts p Gl -> False) /\ (ishParts q Gl -> False) /\ 
-    Forall2 (fun u v => (u = None /\ v = None) \/ (exists p q lis s g, u = Some (gtt_send p q lis) /\ onth l lis = Some(s, g) /\ v = Some g)) ctxG ctxG2.
+    projectableA G ->
+    exists LP LQ S S' T T',
+    projectionC G p (ltt_send q LP) /\ 
+    projectionC G q (ltt_recv p LQ) /\
+    onth l LP = Some(S, T) /\ onth l LQ = Some(S', T').
 Proof.
   intros.
-  specialize(balanced_to_tree G p H); intros.
-Admitted.
+  specialize(wfgC_step_part G G' p q l H H0); intros.
+  specialize(balanced_to_tree G p H H2); intros. clear H2.
+  destruct H3 as (Gl,(ct,(Ha,(Hb,(Hc,Hd))))). clear Hd.
+  revert H H0 H1 Ha Hb Hc. revert G G' p q l ct.
+  induction Gl using gtth_ind_ref; intros.
+  - inversion Ha. subst.
+    specialize(some_onth_implies_In n ct G H4); intros.
+    specialize(Forall_forall (fun u : option gtt =>
+        u = None \/
+        (exists (q : string) (lsg : list (option (sort * gtt))),
+           u = Some (gtt_send p q lsg) \/ u = Some (gtt_send q p lsg) \/ u = Some gtt_end)) ct); intros.
+    destruct H3. specialize(H3 Hc). clear Hc H5.
+    specialize(H3 (Some G) H2). destruct H3; try easy.
+    destruct H3 as (q1,(lsg,Hc)). clear H2.
+    - destruct Hc. inversion H2. subst.  
+      pinversion H0; try easy. subst.
+      unfold projectableA in H1. pose proof H1 as Ht.
+      specialize(H1 p). destruct H1. pinversion H1; try easy. subst.
+      assert False. apply H3. apply triv_pt_p; try easy. easy.
+      subst. specialize(Ht q). destruct Ht. pinversion H3; try easy. 
+      subst. assert False. apply H5. apply triv_pt_q; try easy. easy. subst.
+      exists ys. exists ys0.
+      assert(exists (S S' : sort) (T T' : ltt),
+        onth l ys = Some (S, T) /\ onth l ys0 = Some (S', T')).
+      {
+        clear H16 H18 H15 H9 H13 H7 H3 H8 H11 H4 Hb H2 Ha H1 H0 H.
+        revert H19 H14 H12.
+        revert G' p q lsg ys s ys0. clear n ct.
+        induction l; intros.
+        - destruct lsg; try easy. 
+          destruct ys; try easy. destruct ys0; try easy.
+          inversion H19. subst. clear H19. inversion H14. subst. clear H14.
+          simpl in H12. subst.
+          destruct H2; try easy. destruct H as (s1,(g1,(t1,(Ha,(Hb,Hc))))). inversion Ha. subst.
+          destruct H3; try easy. destruct H as (s2,(g2,(t2,(Hd,(He,Hf))))). inversion Hd. subst.
+          simpl. exists s2. exists s2. exists t2. exists t1. easy.
+        - destruct lsg; try easy. 
+          destruct ys; try easy. destruct ys0; try easy.
+          inversion H19. subst. clear H19. inversion H14. subst. clear H14.
+          specialize(IHl G' p q lsg ys s ys0). apply IHl; try easy.
+      }
+      destruct H5 as (s1,(s2,(t1,(t2,(Hl,Hk))))). exists s1. exists s2. exists t1. exists t2. 
+      split. pfold. easy. split. pfold. easy. easy.
+    apply proj_mon. apply proj_mon. apply step_mon.
+    - destruct H2. inversion H2. subst. pinversion H0; try easy. apply step_mon.
+    - inversion H2. subst. pinversion H0; try easy. apply step_mon.
+  - inversion Ha. subst.
+    clear Ha. rename p into s. rename q into s'. rename p0 into p. rename q0 into q.
+    specialize(proj_forward s s' ys H0 H2); intros. 
+    pinversion H1; try easy. subst. assert False. apply Hb. constructor. easy.
+    subst.
+    specialize(wfgC_after_step_all H10 H0); intros. rename H1 into Htt.
+    clear H19.
+    unfold projectableA in H2. pose proof H2 as Ht.
+    specialize(H2 p). destruct H2 as (T,H2). specialize(Ht q). destruct Ht as (T',Ht).
+    specialize(slist_implies_some xs H8); intros.
+    destruct H1 as (n,(gl,H1)). destruct gl.
+    specialize(Forall2_prop_r n xs ys (s0, g) (fun (u : option (sort * gtth)) (v : option (sort * gtt)) =>
+        u = None /\ v = None \/
+        (exists (s : sort) (g : gtth) (g' : gtt),
+           u = Some (s, g) /\ v = Some (s, g') /\ typ_gtth ct g g')) H1 H9); intros.
+    destruct H5 as (p1,(Hd,He)). destruct He; try easy.
+    destruct H5 as (s1,(g1,(g2,(Hf,(Hg,Hh))))). inversion Hf. subst. clear Hf.
+    specialize(Forall_prop n ys (s1, g2) (fun u : option (sort * gtt) =>
+        u = None \/ (exists (st : sort) (g : gtt), u = Some (st, g) /\ wfgC g)) Hg H4); intros.
+    destruct H5; try easy. destruct H5 as (s2,(g3,(Hi,Hj))). inversion Hi. subst. clear Hi.
+    clear H9 H4 H8.
+    specialize(Forall2_prop_r n ys ys0 (s2, g3) (fun u v : option (sort * gtt) =>
+         u = None /\ v = None \/
+         (exists (s : sort) (g g' : gtt),
+            u = Some (s, g) /\ v = Some (s, g') /\ upaco5 gttstep bot5 g g' p q l)) Hg H20); intros.
+    destruct H4 as (p1,(Hi,Hk)). destruct Hk; try easy. destruct H4 as (s3,(g4,(g5,(Hl,(Hm,Hn))))).
+    inversion Hl. subst. clear Hl H20.
+    specialize(Forall_prop n ys (s3, g4) (fun u : option (sort * gtt) =>
+        u = None \/ (exists (s : sort) (g : gtt), u = Some (s, g) /\ projectableA g)) Hg H3); intros.
+    destruct H4; try easy. destruct H4 as (s4,(g6,(Ho,Hp))). inversion Ho. subst. clear H3.
+    specialize(some_onth_implies_In n xs (s4, g1) H1); intros.
+    specialize(Forall_forall (fun u : option (sort * gtth) =>
+       u = None \/
+       (exists (s : sort) (g : gtth),
+          u = Some (s, g) /\
+          (forall (G G' : gtt) (p q : string) (l : fin) (ct : list (option gtt)),
+           wfgC G ->
+           gttstepC G G' p q l ->
+           projectableA G ->
+           typ_gtth ct g G ->
+           (ishParts p g -> False) ->
+           Forall
+             (fun u0 : option gtt =>
+              u0 = None \/
+              (exists (q0 : string) (lsg : list (option (sort * gtt))),
+                 u0 = Some (gtt_send p q0 lsg) \/ u0 = Some (gtt_send q0 p lsg) \/ u0 = Some gtt_end))
+             ct ->
+           exists (LP LQ : list (option (sort * ltt))) (S S' : sort) (T T' : ltt),
+             projectionC G p (ltt_send q LP) /\
+             projectionC G q (ltt_recv p LQ) /\ onth l LP = Some (S, T) /\ onth l LQ = Some (S', T')))) xs); intros. 
+    destruct H4. specialize(H4 H). clear H H5.
+    specialize(H4 (Some (s4, g1)) H3). destruct H4; try easy.
+    destruct H as (s5,(g7,(Hq,Hr))). inversion Hq. subst.
+    clear H3.
+    specialize(Hr g6 g5 p q l ct).
+    assert(exists (LP LQ : list (option (sort * ltt))) (S S' : sort) (T T' : ltt),
+       projectionC g6 p (ltt_send q LP) /\
+       projectionC g6 q (ltt_recv p LQ) /\ onth l LP = Some (S, T) /\ onth l LQ = Some (S', T')).
+    {
+      apply Hr; try easy.
+      destruct Hn; try easy.
+      specialize(ishParts_n Hb H1); intros. apply H; try easy.
+    }
+    clear Hr. 
+    clear Hp Hn Hm Hj Hh Ho H1 Hq. clear g7 g5.
+    destruct H as (lp,(lq,(s1,(s2,(t1,(t2,(Hta,(Htb,(Htc,Htd))))))))).
+    clear Htt.
+    assert(isgPartsC p g6). 
+    {
+      pinversion Hta; try easy.
+      apply proj_mon.
+    }
+    assert(isgPartsC q g6).
+    {
+      pinversion Htb; try easy.
+      apply proj_mon.
+    }
+    specialize(part_cont_b n ys s5 g6 p s s' Hg); intros.
+    assert(isgPartsC p (gtt_send s s' ys)). apply H3; try easy.
+    specialize(part_cont_b n ys s5 g6 q s s' Hg); intros.
+    assert(isgPartsC q (gtt_send s s' ys)). apply H5; try easy.
+    clear H3 H5.
+    pinversion Ht; try easy. subst. pinversion H2; try easy. subst.
+    clear H23 H22 H19 H18 H17 H16 H15 H6 H4 H1 H H14 H13 H12 H11 H10 H7 Hc Hb.
+    specialize(Forall2_prop_r n ys ys1 (s5, g6) (fun (u : option (sort * gtt)) (v : option ltt) =>
+         u = None /\ v = None \/
+         (exists (s : sort) (g : gtt) (t : ltt),
+            u = Some (s, g) /\ v = Some t /\ upaco3 projection bot3 g q t)) Hg H20); intros.
+    destruct H as (p1,(Ha,Hb)). destruct Hb; try easy. destruct H as (s3,(g1,(t3,(Hb,(Hc,Hd))))).
+    inversion Hb. subst. clear Hb.
+    specialize(Forall2_prop_r n ys ys2 (s3, g1) (fun (u : option (sort * gtt)) (v : option ltt) =>
+         u = None /\ v = None \/
+         (exists (s : sort) (g : gtt) (t : ltt),
+            u = Some (s, g) /\ v = Some t /\ upaco3 projection bot3 g p t)) Hg H26); intros.
+    destruct H as (p2,(He,Hf)). destruct Hf; try easy. destruct H as (s4,(g2,(t4,(Hj,(Hh,Hi))))).
+    inversion Hj. subst.
+    pclearbot.
+    specialize(wfgC_after_step_all H9 H0); intros.
+    specialize(Forall_prop n ys (s4, g2) (fun u : option (sort * gtt) =>
+       u = None \/ (exists (st : sort) (g : gtt), u = Some (st, g) /\ wfgC g)) Hg H); intros.
+    destruct H1; try easy. destruct H1 as (s5,(g3,(Hk,Hl))). inversion Hk. subst.
+    specialize(proj_inj Hl Hi Hta); intros. subst.
+    specialize(proj_inj Hl Hd Htb); intros. subst.
+    clear H H26 H20 Hi Hd.
+    specialize(merge_send_T n T ys2 q lp H27 Hh); intros. destruct H as (lp',H). subst.
+    specialize(merge_recv_T n T' ys1 p lq H21 Hc); intros. destruct H as (lq',H). subst.
+    exists lp'. exists lq'. 
+    specialize(merge_label_recv ys1 lq' lq (s2, t2) n l p H21 Hc Htd); intros. destruct H as (ta,H). 
+    specialize(merge_label_send ys2 lp' lp (s1, t1) n l q H27 Hh Htc); intros. destruct H1 as (tb,H1).
+    destruct ta. destruct tb.
+    exists s3. exists s0. exists l1. exists l0.
+    split. pfold. easy. split. pfold. easy. easy.
+  apply proj_mon.
+  apply proj_mon.
+  apply step_mon.
+Qed.
+
+Lemma proj_cont_pq_step_full : forall G G' p q l,
+    wfgC G -> 
+    gttstepC G G' p q l -> 
+    projectableA G ->
+    exists (T T' : ltt), projectionC G' p T /\ projectionC G' q T'.
+Proof.
+  intros.
+  specialize(proj_cont_pq_step G G' p q l H H0 H1); intros.
+  destruct H2 as (l1,(l2,(s1,(s2,(t1,(t2,(Ha,(Hb,(Hc,Hd))))))))).
+  specialize(_3_19_1_helper p q l G G' l1 l2 s1 t1 s2 t2); intros.
+  exists t1.
+  specialize(_3_19_2_helper p q l G G' l1 l2 s1 t1 s2 t2); intros.
+  exists t2.
+  split. apply H2; try easy. apply H3; try easy.
+Qed.
+
+Lemma nil_word : forall G, exists tc, gttmap G nil None tc.
+Proof.
+  intros.
+  destruct G.
+  exists gnode_end. constructor.
+  exists (gnode_pq s s0). constructor.
+Qed.
+
+Lemma word_step_back_s : forall [w G G' tc p q l], 
+    gttstepC G G' p q l ->
+    gttmap G' w None tc ->
+    gttmap G w None tc \/ (exists w0 w1, w = (w0 ++ w1) /\ gttmap G (w0 ++ l :: w1) None tc /\ gttmap G w0 None (gnode_pq p q)).
+Proof.
+  induction w; intros.
+  - pinversion H.
+    - subst. right. exists nil. exists nil. split. easy.
+      simpl. split. apply gmap_con with (st := s) (gk := G'); try easy.
+      constructor.
+    - subst. left. inversion H0; try easy. subst. constructor.
+    apply step_mon.
+  - pinversion H.
+    - subst. right. exists nil. exists (a :: w).
+      split. easy. split. apply gmap_con with (st := s) (gk := G'); try easy.
+      constructor.
+    - subst.
+      inversion H0. subst. clear H7.
+      specialize(Forall2_prop_l a xs ys (st, gk) (fun u v : option (sort * gtt) =>
+        u = None /\ v = None \/
+        (exists (s : sort) (g g' : gtt),
+           u = Some (s, g) /\ v = Some (s, g') /\ upaco5 gttstep bot5 g g' p q l)) H16 H8); intros.
+      destruct H7 as (p1,(Ha,Hb)). destruct Hb; try easy.
+      destruct H7 as (s1,(g1,(g2,(Hb,(Hc,Hd))))). inversion Hc. subst.
+      destruct Hd; try easy.
+      specialize(IHw g1 g2 tc p q l H7 H17).
+      destruct IHw.
+      - left. apply gmap_con with (st := s1) (gk := g1); try easy.
+      - right.
+        destruct H9 as (w0,(w1,(Hd,He))). subst.
+        exists (a :: w0). exists w1. split. easy.
+        split.
+        apply gmap_con with (st := s1) (gk := g1); try easy.
+        apply gmap_con with (st := s1) (gk := g1); try easy.
+      apply step_mon.
+Qed.
 
 
+Lemma word_step_back_ss : forall [w G G' tc p q l], 
+    gttstepC G G' p q l ->
+    gttmap G' w None tc ->
+    (forall w0 w1 tc1, w = w0 ++ w1 -> (gttmap G' w0 None tc1 <-> gttmap G w0 None tc1)) \/ 
+    (exists w0 w1, w = (w0 ++ w1) /\ 
+    (forall s1 s2 s3 tc1, w0 = s1 ++ s2 ++ (s3 :: nil) -> (gttmap G' s1 None tc1 <-> gttmap G s1 None tc1)) /\
+    (forall s1 s2 tc1, w1 = s1 ++ s2 -> (gttmap G' (w0 ++ s1) None tc1 <-> gttmap G (w0 ++ l :: s1) None tc1)) 
+     /\ gttmap G w0 None (gnode_pq p q)).
+Proof.
+  induction w; intros.
+  - pinversion H.
+    - subst. right. exists nil. exists nil. split. easy.
+      - split. intros. destruct s1; try easy. destruct s2; try easy.
+      - split. intros. destruct s1; try easy. simpl in *.
+        split.
+        - intros.
+          apply gmap_con with (st := s) (gk := G'); try easy.
+        - intros. inversion H4. subst.
+          specialize(eq_trans H2 H12); intros. inversion H3. subst. easy.
+      - constructor. 
+    - subst. left. inversion H0; try easy. subst.
+      intros. split.
+      - intros. destruct w0; try easy. inversion H10; try easy. subst. constructor.
+      - intros. destruct w0; try easy. inversion H10; try easy. 
+    apply step_mon.
+  - pinversion H.
+    - subst. right. exists nil. exists (a :: w).
+      split. easy.
+      - split. intros. destruct s1; try easy. destruct s2; try easy.
+      - split. intros.
+        split.
+        - intros. apply gmap_con with (st := s) (gk := G'); try easy.
+        - intros. inversion H4. subst.
+          specialize(eq_trans H2 H12); intros. inversion H5. subst. easy.
+      - constructor.
+    - subst.
+      inversion H0. subst. clear H7.
+      specialize(Forall2_prop_l a xs ys (st, gk) (fun u v : option (sort * gtt) =>
+        u = None /\ v = None \/
+        (exists (s : sort) (g g' : gtt),
+           u = Some (s, g) /\ v = Some (s, g') /\ upaco5 gttstep bot5 g g' p q l)) H16 H8); intros.
+      destruct H7 as (p1,(Ha,Hb)). destruct Hb; try easy.
+      destruct H7 as (s1,(g1,(g2,(Hb,(Hc,Hd))))). inversion Hc. subst.
+      destruct Hd; try easy.
+      specialize(IHw g1 g2 tc p q l H7 H17).
+      destruct IHw.
+      - left.
+        intros. split. intros. destruct w0. 
+        - inversion H11. subst. constructor.
+        - inversion H10. subst.
+          inversion H11. subst.
+          specialize(eq_trans (eq_sym H21) H16); intros. inversion H12. subst.
+          specialize(H9 w0 w1 tc1).
+          assert(gttmap g1 w0 None tc1). apply H9; try easy.
+          apply gmap_con with (st := s1) (gk := g1); try easy.
+        intros. destruct w0.
+        - inversion H11. subst. constructor.
+        - inversion H10. subst.
+          inversion H11. subst.
+          specialize(eq_trans (eq_sym H21) Hb); intros. inversion H12. subst.
+          specialize(H9 w0 w1 tc1).
+          assert(gttmap g2 w0 None tc1). apply H9; try easy.
+          apply gmap_con with (st := s1) (gk := g2); try easy.
+      - right.
+        destruct H9 as (w0,(w1,(Hd,He))). subst.
+        exists (a :: w0). exists w1. split. easy.
+        destruct He as (He,(Hf,Hg)).
+        - split. intros. 
+          destruct s0. split. intros.
+          - inversion H10. subst. constructor.
+          - intros. inversion H10. subst. constructor.
+          - inversion H9. subst.
+          split. intros. inversion H10. subst. 
+            specialize(eq_trans (eq_sym H20) H16); intros. inversion H11. subst.
+            specialize(He s0 s2 s3 tc1).
+            assert(gttmap g1 s0 None tc1). apply He; try easy.
+            apply gmap_con with (st := s1) (gk := g1); try easy.
+          - intros. inversion H10. subst.
+            specialize(eq_trans (eq_sym H20) Hb); intros. inversion H11. subst.
+            specialize(He s0 s2 s3 tc1).
+            assert(gttmap g2 s0 None tc1). apply He; try easy.
+            apply gmap_con with (st := s1) (gk := g2); try easy.
+        - split. intros.
+          specialize(Hf s0 s2 tc1).
+          split. intros.
+            inversion H10. subst. specialize(eq_trans (eq_sym H20) H16); intros. inversion H9. subst.
+            assert(gttmap g1 (w0 ++ l :: s0) None tc1). apply Hf; try easy.
+            apply gmap_con with (st := s1) (gk := g1); try easy.
+          - intros.
+            inversion H10. subst. specialize(eq_trans (eq_sym H20) Hb); intros. inversion H9. subst.
+            assert(gttmap g2 (w0 ++ s0) None tc1). apply Hf; try easy.
+            apply gmap_con with (st := s1) (gk := g2); try easy.
+          - apply gmap_con with (st := s1) (gk := g1); try easy.
+      apply step_mon.
+Qed.
+
+Lemma decon_word {A} : forall (w2 : list A) l w0 w1 w3,
+    w0 ++ l :: w1 = w2 ++ w3 -> 
+    w0 = w2 \/ (exists wi wj, w0 = w2 ++ wi ++ (wj :: nil)) \/ (exists wi wj, w1 = wi ++ wj /\ w2 = w0 ++ l :: wi).
+Proof.
+  induction w2; intros.
+  - destruct w0. left. easy.
+    right. simpl. left. 
+    clear H. revert a. induction w0; intros. exists nil. exists a. easy.
+    specialize(IHw0 a). destruct IHw0 as (wi,(wj,Ha)). exists (a0 :: wi). exists wj. 
+    replace (a :: w0) with (wi ++ wj :: nil) in *. constructor.
+  - destruct w0.
+    simpl. right. right. inversion H. subst. exists w2. exists w3. easy.
+    inversion H. subst. clear H.
+    specialize(IHw2 l w0 w1 w3 H2).
+    destruct IHw2. left. subst. easy.
+    destruct H.
+    - destruct H as (wi,(wj,Ha)). right. left. exists wi. exists wj. subst. easy.
+    - destruct H as (wi,(wj,Ha)). right. right. destruct Ha. subst.
+      exists wi. exists wj. easy.
+Qed.
+
+Lemma inj_gttmap : forall [w G tc1 tc2], gttmap G w None tc1 -> gttmap G w None tc2 -> tc1 = tc2.
+Proof.
+  induction w; intros.
+  - inversion H. subst. inversion H0. subst. easy.
+    subst. inversion H0. subst. easy.
+  - inversion H. subst.
+    inversion H0. subst.
+    specialize(eq_trans (eq_sym H4) H10); intros. inversion H1. subst.
+    specialize(IHw gk0 tc1 tc2 H7 H11). subst. easy.
+Qed.
+
+Lemma stword {A} : forall w2 wi (wj : A) w1,
+    (w2 ++ wi ++ wj :: nil) ++ w1 = w2 ++ wi ++ wj :: w1.
+Proof.
+  intros.
+  specialize(app_assoc w2 wi (wj :: w1)); intros.
+  apply eq_trans with (y := (w2 ++ wi) ++ wj :: w1); try easy. clear H.
+  specialize(app_assoc w2 wi (wj :: nil)); intros.
+  replace (w2 ++ wi ++ wj :: nil) with ((w2 ++ wi) ++ wj :: nil) in *. clear H.
+  specialize(app_assoc (w2 ++ wi) (wj :: nil) w1); intros.
+  replace (((w2 ++ wi) ++ wj :: nil) ++ w1) with ((w2 ++ wi) ++ (wj :: nil) ++ w1) in *. clear H.
+  constructor.
+Qed.
+
+Lemma cut_word {A} : forall (w : list A) k k',
+    k <= k' -> 
+    length w = k' ->
+    exists w' w2, length w' = k /\ w = w' ++ w2.
+Proof.
+  induction w; intros.
+  - destruct k'; try easy. 
+    destruct k; try easy. exists nil. exists nil. easy.
+  - destruct k'; try easy.
+    destruct k.
+    - exists nil. exists (a :: w). easy.
+    - specialize(IHw k k').
+      assert(exists w' w2 : list A, length w' = k /\ w = w' ++ w2).
+      {
+        apply IHw; try easy. 
+        apply le_S_n; try easy.
+        simpl in H0.
+        apply eq_add_S; try easy.
+      }
+      destruct H1 as (w1,(w2,(Ha,Hb))).
+      exists (a :: w1). exists w2. subst. easy.
+Qed.
+
+Lemma map_back_word : forall [w0 G w1 tc],
+    gttmap G (w0 ++ w1) None tc -> 
+    exists tc, gttmap G w0 None tc.
+Proof.
+  induction w0; intros.
+  - destruct G.
+    - exists gnode_end. constructor.
+    - exists (gnode_pq s s0). constructor.
+  - inversion H. subst.
+    specialize(IHw0 gk w1 tc H6). destruct IHw0 as (tc1,H1).
+    exists tc1.
+    apply gmap_con with (st := st) (gk := gk); try easy.
+Qed.
+
+Lemma cut_further : forall k k' G p0,
+    k <= k' -> 
+    (forall w'0 : list fin,
+     gttmap G w'0 None gnode_end \/
+     length w'0 = k /\ (exists tc : gnode, gttmap G w'0 None tc) ->
+     exists w2 w0 : list fin,
+       w'0 = w2 ++ w0 /\
+       (exists r : string,
+          gttmap G w2 None (gnode_pq p0 r) \/ gttmap G w2 None (gnode_pq r p0))) ->
+    (forall w'0 : list fin,
+     gttmap G w'0 None gnode_end \/
+     length w'0 = k' /\ (exists tc : gnode, gttmap G w'0 None tc) ->
+     exists w2 w0 : list fin,
+       w'0 = w2 ++ w0 /\
+       (exists r : string,
+          gttmap G w2 None (gnode_pq p0 r) \/ gttmap G w2 None (gnode_pq r p0))).
+Proof.
+  intros.
+  destruct H1.
+  - specialize(H0 w'0). apply H0. left. easy.
+  - destruct H1 as (H1,(tc,H2)). rename w'0 into w.
+    specialize(cut_word w k k' H H1); intros.
+    destruct H3 as (w0,(w1,(Ha,Hb))).
+    specialize(H0 w0). subst.
+    assert(gttmap G w0 None gnode_end \/
+     length w0 = length w0 /\ (exists tc : gnode, gttmap G w0 None tc)).
+    {
+      right. split. easy.
+      apply map_back_word with (w1 := w1) (tc := tc); try easy.
+    }
+    specialize(H0 H1). clear H1.
+    destruct H0 as (w2,(w3,(Ha,(r,Hb)))). subst.
+    exists w2. exists (w3 ++ w1). split. apply eq_sym. apply app_assoc.
+    exists r. easy.
+Qed.
 
 Lemma balanced_step : forall [G G' p q l],
     wfgC G -> 
@@ -106,13 +461,290 @@ Lemma balanced_step : forall [G G' p q l],
     projectableA G ->
     balancedG G'.
 Proof.
-  intros.
-  specialize(step_gtth G G' p q l H H0); intros.
+  intros. pose proof H as Ht.
   unfold wfgC in H. destruct H as (Gl,(Ha,(Hb,(Hc,H)))). clear Ha Hb Hc. clear Gl.
-  destruct H2 as (ctxG,(ctxG2,(Gl,(Ha,(Hb,(Hc,(Hd,He))))))).
-  
-  
-Admitted.
+  specialize(wfgC_step_part G G' p q l Ht H0); intros.
+  specialize(balanced_to_tree G p Ht H2); intros.
+  destruct H3 as (Gl,(ct,(Ha,(Hb,(Hc,Hd))))). clear Hd H2.
+  revert Hc Hb Ha Ht H1 H0. clear H.
+  revert G G' p q l ct.
+  induction Gl using gtth_ind_ref; intros; try easy.
+  - inversion Ha. subst.
+    specialize(some_onth_implies_In n ct G H3); intros.
+    specialize(Forall_forall (fun u : option gtt =>
+        u = None \/
+        (exists (q : string) (lsg : list (option (sort * gtt))),
+           u = Some (gtt_send p q lsg) \/ u = Some (gtt_send q p lsg) \/ u = Some gtt_end)) ct); intros.
+    destruct H2. specialize(H2 Hc). clear H4 Hc.
+    specialize(H2 (Some G) H). destruct H2; try easy.
+    destruct H2 as (q1,(lsg,Hc)).
+    - destruct Hc. inversion H2. subst.
+      pinversion H0; try easy. subst.
+      unfold wfgC in Ht. destruct Ht as (G1,(Hta,(Htb,(Htc,Htd)))).
+      specialize(balanced_cont Htd); intros.
+      specialize(some_onth_implies_In l lsg (s, G') (eq_sym H12)); intros.
+      specialize(Forall_forall (fun u : option (sort * gtt) =>
+        u = None \/ (exists (s : sort) (g : gtt), u = Some (s, g) /\ balancedG g)) lsg); intros. 
+      destruct H6. specialize(H6 H4). clear H4 H7.
+      specialize(H6 (Some (s, G')) H5). destruct H6; try easy.
+      destruct H4 as (s1,(g1,(Hsa,Hsb))). inversion Hsa. subst. easy.
+      apply step_mon.
+    - destruct H2. inversion H2. subst. pinversion H0; try easy.
+      apply step_mon.
+    - inversion H2. subst. pinversion H0; try easy.
+      apply step_mon.
+  - inversion Ha. subst. 
+    pinversion H0; try easy.
+    - subst. assert False. apply Hb. constructor. easy.
+    subst. rename p into s. rename q into s'. rename p0 into p. rename q0 into q.
+    assert(Forall (fun u => u = None \/ (exists s g, u = Some(s, g) /\ balancedG g)) ys0).
+    {
+      clear Ha H7. 
+      specialize(wfgC_after_step_all H6 Ht); intros.
+      specialize(proj_forward s s' ys Ht H1); intros. clear H1.
+      clear H5 H6 H9 H10 H11 H12 Ht H0 H17.
+      revert H3 H2 H18 H8 Hc H Hb. revert s s' xs p q l ct ys.
+      induction ys0; intros; try easy.
+      destruct ys; try easy. destruct xs; try easy.
+      inversion H3. subst. clear H3. inversion H2. subst. clear H2.
+      inversion H18. subst. clear H18. 
+      inversion H8. subst. clear H8. inversion H. subst. clear H.
+      specialize(IHys0 s s' xs p q l ct ys).
+      assert(Forall
+          (fun u : option (sort * gtt) =>
+           u = None \/ (exists (s : sort) (g : gtt), u = Some (s, g) /\ balancedG g)) ys0).
+      {
+        apply IHys0; try easy.
+        specialize(ishParts_hxs Hb); try easy.
+      }
+      constructor; try easy.
+      clear H H8 H12 H10 H6 H5 IHys0.
+      destruct H7. left. easy.
+      destruct H as (s1,(g1,(g2,(Hd,(He,Hf))))). subst.
+      destruct H3; try easy. destruct H as (s2,(g3,(Hg,Hh))). inversion Hg. subst.
+      destruct H4; try easy. destruct H as (s3,(g4,(Hi,Hj))). inversion Hi. subst.
+      destruct H9; try easy. destruct H as (s4,(g5,(g6,(Hk,(Hl,Hm))))). inversion Hl. subst.
+      destruct H2; try easy. destruct H as (s5,(g7,(Hn,Ho))). inversion Hn. subst.
+      right. exists s5. exists g2. split. easy.
+      clear Hn Hl Hg Hi. destruct Hf; try easy. 
+      specialize(Ho g6 g2 p q l ct). apply Ho; try easy.
+      specialize(ishParts_x Hb); try easy.
+    }
+    clear H18 H17 H8 H7 H.
+    unfold balancedG.
+    intros.
+    destruct w.
+    - simpl.
+      {
+        simpl in *. 
+        assert(exists Gl, Gl = (gtth_send s s' xs)). exists (gtth_send s s' xs). easy.
+        destruct H4 as (Gl,H4). replace (gtth_send s s' xs) with Gl in *.
+        assert(exists G, G = (gtt_send s s' ys)). exists (gtt_send s s' ys). easy.
+        destruct H7 as (G,H7). replace (gtt_send s s' ys) with G in *.
+        assert(exists G', G' = (gtt_send s s' ys0)). exists (gtt_send s s' ys0). easy.
+        - case_eq (eqb p0 p); intros.
+          assert (p0 = p). apply eqb_eq; try easy. subst. 
+          {
+            clear H4 Hc Hb Ha. 
+            clear H8 H7 H13.
+            assert(gttstepC G (gtt_send s s' ys0) p q l). pfold. easy. clear H0.
+            specialize(proj_cont_pq_step_full G (gtt_send s s' ys0) p q l Ht H4 H1); intros.
+            destruct H0 as (T,(T1,(Ha,Hb))). clear Hb. clear T1.
+            
+            specialize(wfgCw_after_step G (gtt_send s s' ys0) p q l Ht H4); intros. 
+            clear H4 H12 H11 H10 H9 H6 H5 Ht H1.
+            admit. 
+          }
+        - case_eq (eqb p0 q); intros.
+          assert (p0 = q). apply eqb_eq; try easy. subst. 
+          {
+            admit.
+          }
+        - destruct H8 as (G',H8). replace (gtt_send s s' ys0) with G' in *. clear H4 H7 H8.
+          assert (p0 <> p). apply eqb_neq; try easy. 
+          assert (p0 <> q). apply eqb_neq; try easy.
+          {
+            pose proof Ht as Htt.
+            unfold wfgC in Htt. destruct Htt as (G1,(Hf,(Hg,(Hd,He)))). clear Hf Hg Hd. clear G1.
+            clear H13 H14 H H12 H11 H10 H9 H6 H5 Ht.
+            assert(gttstepC G G' p q l). pfold. easy. clear H0 H1 H2. clear s s' xs ys ys0.
+            unfold balancedG in He. specialize(He nil). simpl in He.
+            
+            assert(exists k : fin,
+       forall w'0 : list fin,
+       gttmap G w'0 None gnode_end \/ length w'0 = k /\ (exists tc : gnode, gttmap G w'0 None tc) ->
+       exists w2 w0 : list fin,
+         w'0 = w2 ++ w0 /\
+         (exists r : string, gttmap G w2 None (gnode_pq p0 r) \/ gttmap G w2 None (gnode_pq r p0))).
+            {
+              specialize(nil_word G); intros.
+              destruct H0 as (tc1,H0).
+              destruct H3.
+              - specialize(word_step_back_s H H1); intros.
+                destruct H2. specialize(He w' p0 q0 tc1). apply He; try easy.
+                left. easy.
+              - destruct H2 as (w0,(w1,(Hd,Hf))). specialize(He (w0 ++ l :: w1) p0 q0 tc1).
+                apply He; try easy.
+                left. easy.
+              - specialize(word_step_back_s H H1); intros.
+                destruct H2. specialize(He w' p0 q0 tc1). apply He; try easy.
+                right. easy.
+              - destruct H2 as (w0,(w1,(Hd,Hf))). specialize(He (w0 ++ l :: w1) p0 q0 tc1).
+                apply He; try easy.
+                right. easy.
+            }
+            clear He H3.
+            
+            destruct H0 as (k, H0). exists k.
+            intros.
+            destruct H1.
+            - specialize(word_step_back_ss H H1); intros.
+              destruct H2.
+              - specialize(H0 w'0).
+                assert(gttmap G w'0 None gnode_end \/ length w'0 = k /\ (exists tc : gnode, gttmap G w'0 None tc)).
+                {
+                  left. specialize(H2 w'0 nil gnode_end). apply H2; try easy.
+                  apply eq_sym.
+                  apply app_nil_r.
+                }
+                specialize(H0 H3). clear H3.
+                destruct H0 as (w2,(w0,(Hta,(r,Htb)))).
+                exists w2. exists w0. split. easy. exists r.
+                destruct Htb.
+                - specialize(H2 w2 w0 (gnode_pq p0 r)). left. apply H2; try easy.
+                - specialize(H2 w2 w0 (gnode_pq r p0)). right. apply H2; try easy.
+              - destruct H2 as (w0,(w1,(Hd,(He,(Hf,Hg))))). subst.
+                pose proof Hf as Ht.
+                specialize(Hf w1 nil gnode_end).
+                assert(gttmap G (w0 ++ l :: w1) None gnode_end). apply Hf; try easy.
+                apply eq_sym. apply app_nil_r.
+                specialize(H0 (w0 ++ l :: w1)).
+                assert(gttmap G (w0 ++ l :: w1) None gnode_end \/
+     length (w0 ++ l :: w1) = k /\ (exists tc : gnode, gttmap G (w0 ++ l :: w1) None tc)). left. easy.
+                specialize(H0 H3). clear H3.
+                destruct H0 as (w2,(w3,(Hh,(r,Hi)))).
+                clear Hc Hb Ha H H1 H2 Hf.
+                specialize(decon_word w2 l w0 w1 w3 Hh); intros.
+                - destruct H.
+                  subst. destruct Hi.
+                  specialize(inj_gttmap Hg H); intros. inversion H0. subst. easy.
+                  specialize(inj_gttmap Hg H); intros. inversion H0. subst. easy.
+                - destruct H.
+                  destruct H as (wi,(wj,Hta)). subst.
+                  specialize(He w2 wi wj). exists w2. exists (wi ++ wj :: w1).
+                  split.
+                  apply stword.
+                  exists r. destruct Hi.
+                  specialize(He (gnode_pq p0 r)). left. apply He; try easy.
+                  specialize(He (gnode_pq r p0)). right. apply He; try easy.
+                - destruct H as (wi,(wj,(Hta,Htb))). subst.
+                  specialize(Ht wi wj). exists (w0 ++ wi). exists wj. split. 
+                  apply app_assoc. exists r.
+                  destruct Hi.
+                  - left. apply Ht; try easy.
+                  - right. apply Ht; try easy.
+          - destruct H1 as (H1,(tc,H2)).
+            specialize(word_step_back_ss H H2); intros.
+            clear Hc Hb Ha H. clear Gl ct. clear w' gn.
+            destruct H3.
+            - assert(gttmap G w'0 None gnode_end \/
+     length w'0 = k /\ (exists tc : gnode, gttmap G w'0 None tc)).
+              {
+                right. split. easy. exists tc.
+                specialize(H w'0 nil). apply H; try easy.
+                apply eq_sym. apply app_nil_r.
+              }
+              specialize(H0 w'0 H3). clear H3.
+              destruct H0 as (w2,(w0,(Ha,(r,Hb)))).
+              subst. exists w2. exists w0. split. easy. exists r.
+              specialize(H w2 w0). destruct Hb.
+              - left. apply H; try easy.
+              - right. apply H; try easy.
+            - destruct H as (w0,(w1,(Ha,(Hb,(Hc,Hd))))).
+              assert(k <= S k). constructor. constructor.
+              specialize(cut_further k (S k) G p0 H H0); intros. clear H H0.
+              assert(gttmap G (w0 ++ l :: w1) None tc).
+              {
+                specialize(Hc w1 nil tc). apply Hc; try easy.
+                apply eq_sym. apply app_nil_r; try easy. subst. easy.
+              }
+              specialize(H3 (w0 ++ l :: w1)).
+              assert(gttmap G (w0 ++ l :: w1) None gnode_end \/
+               length (w0 ++ l :: w1) = S k /\
+               (exists tc : gnode, gttmap G (w0 ++ l :: w1) None tc)).
+              {
+                right. split. subst.
+                clear H H3 Hd Hc Hb H2 H7 H4. clear p q G G' p0 q0 tc.
+                revert w1 l. induction w0; intros; try easy.
+                simpl in *. apply eq_S. apply IHw0; try easy.
+                exists tc. easy.
+              }
+              specialize(H3 H0). clear H0.
+              destruct H3 as (w2,(w3,(He,(r,Hf)))). subst.
+              specialize(decon_word w2 l w0 w1 w3 He); intros.
+              - destruct H0.
+                subst.
+                destruct Hf. 
+                - specialize(inj_gttmap H0 Hd); intros. inversion H1. subst. easy.
+                - specialize(inj_gttmap H0 Hd); intros. inversion H1. subst. easy.
+              - destruct H0.
+                destruct H0 as (wi,(wj,Hg)). subst.
+                specialize(Hb w2 wi wj). exists w2. exists (wi ++ wj :: w1). 
+                split. apply stword.
+                exists r.
+                destruct Hf.
+                - left. apply Hb; try easy.
+                - right. apply Hb; try easy.
+              - destruct H0 as (wi,(wj,(Hg,Hh))). subst.
+                specialize(Hc wi wj).
+                exists (w0 ++ wi). exists wj. split. apply app_assoc.
+                exists r.
+                destruct Hf.
+                - left. apply Hc; try easy.
+                - right. apply Hc; try easy.
+            }
+      }
+    - inversion H. subst.
+      specialize(some_onth_implies_In n ys0 (st, gk) H17); intros.
+      specialize(Forall_forall (fun u : option (sort * gtt) =>
+        u = None \/ (exists (s : sort) (g : gtt), u = Some (s, g) /\ balancedG g)) ys0); intros.
+      destruct H7. specialize(H7 H2). clear H8 H2.
+      specialize(H7 (Some (st, gk)) H4). destruct H7; try easy.
+      destruct H2 as (s1,(g1,(Hta,Htb))). inversion Hta. subst. clear H4 Hta.
+      unfold balancedG in Htb.
+      specialize(Htb w w' p0 q0 gn H18).
+      assert(gttmap g1 (seq.cat w w') None (gnode_pq p0 q0) \/ gttmap g1 (seq.cat w w') None (gnode_pq q0 p0)).
+      {
+        destruct H3. left. inversion H2; try easy. subst. specialize(eq_trans (eq_sym H16) H17); intros.
+        inversion H3. subst. easy.
+        right. inversion H2; try easy. subst. specialize(eq_trans (eq_sym H16) H17); intros.
+        inversion H3. subst. easy.
+      }
+      specialize(Htb H2). clear H2 H3.
+      destruct Htb. exists x. intros.
+      specialize(H2 w'0).
+      assert(gttmap g1 (seq.cat w w'0) None gnode_end \/
+     length w'0 = x /\ (exists tc : gnode, gttmap g1 (seq.cat w w'0) None tc)).
+      {
+        destruct H3. left.
+        inversion H3. subst. specialize(eq_trans (eq_sym H19) H17); intros. inversion H4. subst.
+        easy.
+        destruct H3. destruct H4 as (tc, H4).
+        right. split; try easy.
+        exists tc. inversion H4. subst.
+        specialize(eq_trans (eq_sym H20) H17); intros. inversion H3. subst.
+        easy.
+      }
+      specialize(H2 H4).
+      destruct H2 as (w2,(w0,(Hsa,Hsb))). exists w2. exists w0.
+      split. easy. destruct Hsb as (r, Hsb). exists r.
+      {
+        destruct Hsb.
+        left. apply gmap_con with (st := s1) (gk := g1); try easy.
+        right. apply gmap_con with (st := s1) (gk := g1); try easy.
+      }
+    apply step_mon.
+Admitted. 
 
 Theorem wfgC_after_step : forall G G' p q n, wfgC G -> gttstepC G G' p q n -> projectableA G -> wfgC G'. 
 Proof.
